# Base vocabulary for (UK) public sector bodies, building upon generic org vocab
# Design use cases:
#     - core metadata - type, name
#     - contact information
#     - senior executives
#     - link to organizational sub-structure and associated services
#       (neutral to the details and terminology for that structure) 

@prefix rdf:            <http://www.w3.org/1999/02/22-rdf-syntax-ns#> .
@prefix rdfs:           <http://www.w3.org/2000/01/rdf-schema#> .
@prefix owl:            <http://www.w3.org/2002/07/owl#> .
@prefix vs:             <http://www.w3.org/2003/06/sw-vocab-status/ns#> .
@prefix xsd:            <http://www.w3.org/2001/XMLSchema#> .
@prefix skos:           <http://www.w3.org/2004/02/skos/core#> .
@prefix foaf:           <http://xmlns.com/foaf/0.1/> .
@prefix void:           <http://rdfs.org/ns/void#> .
@prefix qb:             <http://purl.org/linked-data/cube#> .
@prefix dcterms:        <http://purl.org/dc/terms/> .
@prefix org:            <http://www.w3.org/ns/org#> .
@prefix vcard:          <http://www.w3.org/2006/vcard/ns#> .
@prefix event:		<http://purl.org/NET/c4dm/event.owl#> .
@prefix statsGeo:       <http://statistics.data.gov.uk/def/administrative-geography/> .
@prefix payment:        <http://reference.data.gov.uk/def/payment#> .
@prefix interval:       <http://reference.data.gov.uk/def/intervals/>.
@prefix gov:		<http://reference.data.gov.uk/def/central-government/> .
@prefix postcode:       <http://data.ordnancesurvey.co.uk/ontology/postcode/postcode> .
@prefix geo:            <http://www.w3.org/2003/01/geo/wgs84_pos#> .
@prefix spatialrelations: <http://data.ordnancesurvey.co.uk/ontology/spatialrelations/> .
@prefix admingeo:       <http://data.ordnancesurvey.co.uk/ontology/admingeo/> .

@prefix psb:  <http://reference.data.gov.uk/def/public-sector-body#> .
@base         <http://reference.data.gov.uk/def/public-sector-body#> .

# -- Meta data -----------------------------------------------------------

<>
    a owl:Ontology;
    owl:versionInfo "0.4";
    rdfs:label "Public Sector Body base ontology"@en;
    rdfs:comment """"Base vocabulary for public sector bodies such as Local Authorities, building upon generic org vocab. Designed to support:
    <ul><li>core metadata - type, name</li>
    <li>contact information</li>
    <li>senior executives</li>
    <li>organizational units with contact details and associated services</li>"""@en;
    dcterms:created  "2010-09-07"^^xsd:date;
    dcterms:modified "2010-10-27"^^xsd:date;
    dcterms:contributor [foaf:mbox "dave@epimorphics.com";  foaf:name "Dave Reynolds"];
    dcterms:license <http://www.opendatacommons.org/licenses/pddl/1.0/> ;
    .

# -- Types of local authority --------------------------------------------------

psb:Body a rdfs:Class, owl:Class;
    rdfs:label "Public sector body"@en;
    rdfs:comment """Any form of public sector budy such as a local authority."""@en;
    rdfs:subClassOf  org:FormalOrganization, foaf:Organization ;
    vs:term_status "proposed";    rdfs:isDefinedBy <> .

psb:LocalAuthority a rdfs:Class, owl:Class;
    rdfs:label "Local authority"@en;
    rdfs:comment """Any form of public sector body with a regional coverage, including county councils, district councils and unitary authorities. 
Relevant descriptive properties to consider include: <ul>
<li>owl:sameAs links to statistics.gov.uk and others as desired (e.g. OpenlyLocal, dbpedia), 
     to link to wikipedia use foaf:isPrimaryTopicOf</li>
<li>rdfs:label</li>
<li>psb:officialName, psb:vernacularName, skos:altLabel</li>
<li>psb:coverage link to the region served</li>
<li>skos:notation "xxxx"^^statsGeo:StandardCode giving the SNAC code</li>
<li>psb:localAuthorityType link to a categorization of the local authority, e.g. as provided by ESDToolit</li>
<li>org:hasPrimarySite with a VCard to give the location and contacts details for the main council site</li>
<li>org:hasSite for other sites</li>
<li>psb:mainPhone, psb:phone, psb:contactForm, psb:contactInformation</li>
<li>foaf:homepage, foaf:mbox, foaf:holdsAccount (if appropriate)</li>
<li>gov:hasPost for senior officers, especially chief execution</li>
<li>org:hasUnit links to organzation units (such as Departments or Directorates)
</ul>"""@en;
    rdfs:subClassOf  psb:Body, statsGeo:LocalAuthority ;
    vs:term_status "proposed";    rdfs:isDefinedBy <> .

psb:localAuthorityType a rdf:Property, owl:ObjectProperty;
    rdfs:label "local authority type"@en;
    rdfs:comment "Gives a classification for the local authority in terms of a controlled list of types"@en;
    rdfs:subPropertyOf org:classification;
    rdfs:domain psb:LocalAuthority;
    rdfs:range skos:Concept;
    vs:term_status "proposed";    rdfs:isDefinedBy <> .

## Codify expected properties --------------------------------------------------
# Here we use minCardinality of 0 to indicate optional properties which might be considered
# and minCardinality 1 to indicate properties that are expected. Note that the open world
# assumption still applies, a minCardinality 1 property can be omitted from any particular
# data set without problems though its omission should be detected as a warning by any 
# lint-like checking tools.

psb:Body
    rdfs:subClassOf [ a owl:Restriction;
        owl:onProperty psb:officialName;
        owl:cardinality 1 ] ;

    rdfs:subClassOf [ a owl:Restriction;
        owl:onProperty psb:vernacularName;
        owl:cardinality 1 ] ;

    rdfs:subClassOf [ a owl:Restriction;
        owl:onProperty org:hasPrimarySite;
        owl:minCardinality 1 ] ;

    rdfs:subClassOf [ a owl:Restriction;
        owl:onProperty org:hasSite;     # for other premises
        owl:minCardinality 0 ] ;        

    rdfs:subClassOf [ a owl:Restriction;
        owl:onProperty foaf:holdsAccount;
        owl:minCardinality 0 ] ;

    rdfs:subClassOf [ a owl:Restriction;
        owl:onProperty foaf:homepage;
        owl:minCardinality 0 ] ;

    rdfs:subClassOf [ a owl:Restriction;
        owl:onProperty psb:contactForm;
        owl:minCardinality 0 ] ;

    rdfs:subClassOf [ a owl:Restriction;
        owl:onProperty psb:contactInformation;
        owl:minCardinality 0 ] ;

    rdfs:subClassOf [ a owl:Restriction;
        owl:onProperty foaf:mbox;
        owl:minCardinality 1 ] ;

    rdfs:subClassOf [ a owl:Restriction;
        owl:onProperty psb:mainPhone;
        owl:minCardinality 0 ] ;

    rdfs:subClassOf [ a owl:Restriction;
        owl:onProperty psb:phone;
        owl:minCardinality 0 ] ;

    rdfs:subClassOf [ a owl:Restriction;
        owl:onProperty foaf:isPrimaryTopicOf;   # For wikipedia links
        owl:minCardinality 0 ] ;

    rdfs:subClassOf [ a owl:Restriction;
        owl:onProperty gov:hasPost ;
        owl:minCardinality 0 ] ;

    rdfs:subClassOf [ a owl:Restriction;
        owl:onProperty org:hasUnit;		# For departments/directorates
        owl:minCardinality 0 ] ;
    .

psb:LocalAuthority
    rdfs:subClassOf [ a owl:Restriction;
        owl:onProperty psb:coverage;
        owl:minCardinality 1 ] ;

    rdfs:subClassOf [ a owl:Restriction;
        owl:onProperty psb:localAuthorityType;
        owl:minCardinality 1 ] ;

    rdfs:subClassOf [ a owl:Restriction;
        owl:onProperty skos:notation;    # for SNAC code
        owl:minCardinality 0 ] ;
    .

# -- naming ----------------------------------------------------------------

psb:officialName a rdf:Property, owl:DatatypeProperty ;
    rdfs:label "official name"@en;
    rdfs:comment "The official name for a body or region, as defined in legislation"@en; 
    rdfs:subPropertyOf rdfs:label;
    .

psb:vernacularName a rdf:Property, owl:DatatypeProperty ;
    rdfs:label "official name"@en;
    rdfs:comment "Commonly used name for a body or region, alternative non-preferred names can be given by skos:altLabel"@en; 
    rdfs:subPropertyOf rdfs:label;
    .

# -- Link to service classifications ---------------------------------------

psb:providesService a rdf:Property, owl:ObjectProperty;
    rdfs:label "provides services"@en;
    rdfs:comment """Indicates a service (described using SKOS) which is
    provided by an organzation or a unit of an organization. """@en;
    rdfs:domain org:Organization;
    rdfs:range  skos:Concept ;	
    vs:term_status "proposed";    rdfs:isDefinedBy <> .

psb:coverage a rdf:Property, owl:ObjectProperty ;
    rdfs:label "coverage"@en;
    rdfs:comment """The administrative area covered by this authority"""@en;
    rdfs:domain  psb:LocalAuthority;
    rdfs:range   admingeo:CivilAdministrativeArea;
    vs:term_status "proposed";    rdfs:isDefinedBy <> .
    
# -- Contact details -----------------------------------------------------------

psb:Contact a rdfs:Class, owl:Class;
    rdfs:label "contact details"@en;
    rdfs:comment """A means of contact including email, phone, mail addresses, physical site. Defined as a
union of the vcard types (Address, Email, Tel) and org:Site. Provided so that contact annotations can
e associated with any of these contact mechanisms."""@en;
    rdfs:subClassOf
         [ a owl:Class ;
             owl:unionOf ( vcard:Address vcard:Email vcard:Tel org:Site )
         ] ;
    .

psb:mainPhone a rdf:Property, owl:ObjectProperty;
    rdfs:label "main phone"@en;
    rdfs:comment "The primary contact phone number, this should be a vcard:Tel using appropriate annotations to describe access information and purpose/coverage information"@en;
    rdfs:range vcard:Tel;
    vs:term_status "proposed";    rdfs:isDefinedBy <> .

psb:phone a rdf:Property, owl:ObjectProperty;
    rdfs:label "phone"@en;
    rdfs:comment "A contact phone number, this should be a vcard:Tel using appropriate annotations to describe access information and purpose/coverage information"@en;
    rdfs:range vcard:Tel;
    vs:term_status "proposed";    rdfs:isDefinedBy <> .

psb:accessInformation a rdf:Property, owl:DatatypeProperty;
    rdfs:label "contact access information"@en;
    rdfs:comment """A textual description of access information for the contact point. 
This might include opening hours or accessibility information."""@en;
    rdfs:domain psb:Contact ;
    vs:term_status "proposed";    rdfs:isDefinedBy <> .

psb:contactPurpose a rdf:Property, owl:DatatypeProperty;
    rdfs:label "contact point purpose"@en;
    rdfs:comment """A textual description of what the purpose of this access point is, 
a description of the type of enquires handled."""@en;
    rdfs:domain psb:Contact ;
    vs:term_status "proposed";    rdfs:isDefinedBy <> .

psb:OutOfHours a rdfs:Class, owl:Class ;
    rdfs:label "out-of-hours number"@en;
    rdfs:comment "A phone number for emergency or out-of-hours contact"@en;
    rdfs:subClassOf vcard:tel;
    vs:term_status "proposed";    rdfs:isDefinedBy <> .

psb:contactForm a rdf:Property, owl:ObjectProperty;
    rdfs:label "contact form"@en;
    rdfs:comment "gives a web contact form for the organization"@en;
    rdfs:domain psb:Body;
    vs:term_status "proposed";    rdfs:isDefinedBy <> .

psb:contactInformation a rdf:Property, owl:ObjectProperty;
    rdfs:label "contact information"@en;
    rdfs:comment "gives a web page listing contact details for the organization"@en;
    rdfs:domain psb:Body;
    vs:term_status "proposed";    rdfs:isDefinedBy <> .

## Location information -----------------------------------------------------

org:Site
    rdfs:subClassOf [ a owl:Restriction;
        owl:onProperty geo:lat;
        owl:minCardinality 0 ] ;

    rdfs:subClassOf [ a owl:Restriction;
        owl:onProperty geo:long;
        owl:minCardinality 0 ] ;

    rdfs:subClassOf [ a owl:Restriction;
        owl:onProperty spatialrelations:easting;
        owl:minCardinality 0 ] ;

    rdfs:subClassOf [ a owl:Restriction;
        owl:onProperty spatialrelations:northing;
        owl:minCardinality 0 ] ;

    rdfs:subClassOf [ a owl:Restriction;
        owl:onProperty psb:accessInformation;
        owl:minCardinality 0 ] ;

    rdfs:subClassOf [ a owl:Restriction;
        owl:onProperty postcode:postcode;
        owl:minCardinality 0 ] ;
    .

# -- Posts for senior officers -----------------------------------------------------------

psb:ChiefExecutive a rdfs:Class, owl:Class;
    rdfs:label "Chief Executive"@en;
    rdfs:comment """Post of Chief Executive. The instances (different for each local authority) should
link to the Authority using gov:postIn and to the individual currently holding the post using gov:heldBy/gov:holdsPost"""@en;
    rdfs:subClassOf gov:Post ;
    vs:term_status "proposed";    rdfs:isDefinedBy <> .

psb:Leader a rdfs:Class, owl:Class;
    rdfs:label "Leader"@en;
    rdfs:comment """Post of council leader. The instances (different for each local authority) should
link to the Authority using gov:postIn and to the individual currently holding the post using gov:heldBy/gov:holdsPost"""@en;
    rdfs:subClassOf gov:Post ;
    vs:term_status "proposed";    rdfs:isDefinedBy <> .

psb:DeputyLeader a rdfs:Class, owl:Class;
    rdfs:label "Deputy Leader"@en;
    rdfs:comment """Post of deputy council leader. The instances (different for each local authority) should
link to the Authority using gov:postIn and to the individual currently holding the post using gov:heldBy/gov:holdsPost"""@en;
    rdfs:subClassOf gov:Post ;
    vs:term_status "proposed";    rdfs:isDefinedBy <> .

psb:Chairman a rdfs:Class, owl:Class;
    rdfs:label "Chairman"@en;
    rdfs:comment """Post of council chairman. The instances (different for each local authority) should
link to the Authority using gov:postIn and to the individual currently holding the post using gov:heldBy/gov:holdsPost"""@en;
    rdfs:subClassOf gov:Post ;
    vs:term_status "proposed";    rdfs:isDefinedBy <> .

psb:Mayor a rdfs:Class, owl:Class;
    rdfs:label "Mayor"@en;
    rdfs:comment """Post of Mayor, covers Lord Mayors and elected Mayors. The instances (different for each local authority) 
link to the Authority using gov:postIn and to the individual currently holding the post using gov:heldBy/gov:holdsPost."""@en;
    rdfs:subClassOf gov:Post ;
    vs:term_status "proposed";    rdfs:isDefinedBy <> .

psb:chiefExecutive a rdf:Property, owl:ObjectProperty;
    rdfs:label "chief executive"@en;
    rdfs:comment "A short cut indicating the person who currently holds the post of Chief Executive of this local authority"@en;
    rdfs:subPropertyOf org:hasMember;
    rdfs:domain psb:LocalAuthority ;
    rdfs:range  foaf:Agent ;
    vs:term_status "proposed";    rdfs:isDefinedBy <> .

